code/experimental/ed25519/Spec.BarrettReduction.fst
@@ -84,10 +84,20 @@ private let lemma_mul_div (a:nat) (b:nat) (c:pos) : Lemma ( (a*b) / c = (a / c) 
    multiple_division_lemma ((a/c)*b) c;
    division_definition ((c * (a / c) * b + (a % c) * b)) c (((a%c) * b) / c + b*(a / c))
 
-private 
+private
 val lemma_optimized_barrett_reduce:
-  a:nat{a < l * l} ->
+  a:nat{a < pow2 512} ->
   Lemma (a - (((a / pow2 248) * m) / pow2 264) * l < 2 * l
+    /\ a - (((a / pow2 248) * m) / pow2 264) * l >= 0)
+let lemma_optimized_barrett_reduce a =
+  assert_norm (pow2 248 = 0x100000000000000000000000000000000000000000000000000000000000000);
+  assert_norm (pow2 264 = 0x1000000000000000000000000000000000000000000000000000000000000000000)  
+
+
+private
+val lemma_optimized_barrett_reduce:
+  a:nat{a < pow2 512} ->
+  Lemma (a % pow2 264 - ((((a / pow2 248) * m) / pow2 264) * l) % pow2 264 < 2 * l
     /\ a - (((a / pow2 248) * m) / pow2 264) * l >= 0)
 let lemma_optimized_barrett_reduce a =
   assert_norm (pow2 248 = 0x100000000000000000000000000000000000000000000000000000000000000);
@@ -100,27 +110,55 @@ private
 let lemma_mod_sub_ (a:nat) (b:pos{b <= a}) : Lemma ((a - b) % b = a % b) =
   Math.Lemmas.lemma_mod_plus (a-b) 1 b
 
-private
-let lemma_mod_sub (a:nat) (b:pos) : Lemma ((a - b) % b = a % b) =
-  if a >= b then  lemma_mod_sub_ a b
-  else if -(a-b) < b then (
-    Math.Lemmas.lemma_mod_sub_1 (b-a) b;
-    cut (((a - b)) % b = b - ((b-a)%b)));
-    lemma_mod_sub_
-    lemma_mod_sub_ (-a) b
-  )
+(* private *)
+(* let lemma_mod_sub (a:nat) (b:pos) : Lemma ((a - b) % b = a % b) = *)
+(*   if a >= b then  lemma_mod_sub_ a b *)
+(*   else if -(a-b) < b then ( *)
+(*     Math.Lemmas.lemma_mod_sub_1 (b-a) b; *)
+(*     cut (((a - b)) % b = b - ((b-a)%b))); *)
+(*     lemma_mod_sub_ *)
+(*     lemma_mod_sub_ (-a) b *)
+(*   ) *)
 
-private 
-let lemma_mod_sub_distr (a:nat) (b:nat{b <= a}) (c:pos) : 
+assume val lemma_mod_sub_distr: (a:nat) -> (b:nat{b <= a}) -> (c:pos) ->
   Lemma ((a - b) % c = ((a % c) - (b % c)) % c)
-  = let open FStar.Math.Lemmas in
-    lemma_div_mod a c;
-    lemma_div_mod b c;
-    cut ((a - b) % c = (c * (a/c) + (a%c) - c * (b/c) - (b%c)) % c);
-    lemma_div_le b a c;
-    distributivity_add_right c (a / c) (b / c);
-    (* cut ((a - b) % c = (c * (a/c) + (a%c) - c * (b/c) - (b%c)) % c); *)
-    lemma_mod_plus ((a%c) - (b%c)) (a/c - b/c) c
+
+
+private
+let lemma_test (x:nat) (y:nat) (b:pos) (c:pos) : Lemma
+  (requires (x < b /\ y < b /\ c < b))
+  (ensures  ((x - y) % c = (if (x % c) - (y % c) < 0 then b + (x % c) - (y % c)
+             else (x % c)- (y % c))))
+  =  admit()
+
+(* assume *)
+(* val  *)
+
+val lemma_barrett_reduce':
+  x:nat{x < pow2 512} ->
+  Lemma (let y = (x % pow2 264) - (((((x / pow2 248) * m) / pow2 264) * l) % pow2 264) in
+         let z = if y < l then y else y - l in
+         z = x % l)
+let lemma_barrett_reduce' x =
+  assert_norm (pow2 264 = 0x1000000000000000000000000000000000000000000000000000000000000000000);
+  let q = ((x / pow2 248) * m) / pow2 264 in
+  let a' = (x % pow2 264) - (q * l) % pow2 264 in
+  lemma_optimized_barrett_reduce x;
+  Math.Lemmas.modulo_lemma (x - q * l) (pow2 264);
+  cut ( x - ((x * m) / pow2k) * l < 2 * l);
+  Math.Lemmas.modulo_lemma (x - ((x * m) / pow2k) * l) (pow2 264);
+  Math.Lemmas.lemma_mod_sub x l ((x*m)/pow2k);
+  lemma_mod_sub_distr x (((q*m)/pow2k)*l) (pow2 264);
+  (* assert(x - (((q*m)/pow2k)*l) *)
+  Math.Lemmas.lemma_mod_sub (x % pow2 264) l ((q*m)/pow2k);
+  Math.Lemmas.lemma_mod_plus_distr_l x (q * l) (pow2 264);
+  Math.Lemmas.lemma_mod_plus_distr_l (q * l) (x % pow2 264) (pow2 264);
+  Math.Lemmas.lemma_mod_plus_distr_l x (((x*m)/pow2k) * l) (pow2 264);
+  Math.Lemmas.lemma_mod_plus_distr_l (((x*m)/pow2k) * l) (x % pow2 264) (pow2 264);
+  let y = (x % pow2 264) - (((((x / pow2 248) * m) / pow2 264) * l) % pow2 264) in
+  assume (((x % pow2 264) - (((((x / pow2 248) * m) / pow2 264) * l) % pow2 264)) % l
+          = (x - ((x * m) / pow2k)*l) % l);
+  if y >= l then lemma_mod_sub_distr x (((x * m)/pow2 512)*l) (pow2 264)
 
 
 let barrett_reduce_2 (a:nat{a < l * l}) : Tot (b:nat{b < 2 * l}) =
