code/experimental/ed25519/Hacl.Spec.BignumQ.Mul.Lemmas_3.fst
@@ -13,23 +13,27 @@ private
 let lemma_distr_4 x a b c d : Lemma (x * (a + b + c + d) = x * a + x * b + x * c + x * d)
   = ()
 
+private
+let lemma_distr_5 x a b c d e : Lemma (x * (a + b + c + d + e) = x * a + x * b + x * c + x * d + x * e)
+ = ()
+
 val lemma_mod_264:
-  x0:u56 -> x1:u56 -> x2:u56 -> x3:u56 -> x4:u56 -> x5:u56 -> x6:u56 -> x7:u56 -> x8:t ->
+  x0:u56 -> x1:u56 -> x2:u56 -> x3:u56 -> x4:u56 -> x5:u56 -> x6:u56 -> x7:u56 -> x8:u56 -> x9:u56 ->
   Lemma ((v x0 + p1 * v x1 + p2 * v x2 + p3 * v x3 + p4 * v x4
-         + p5 * v x5 + p6 * v x6 + p7 * v x7 + p8 * v x8) % pow2 264
+         + p5 * v x5 + p6 * v x6 + p7 * v x7 + p8 * v x8 + p9 * v x9) % pow2 264
          = v x0 + p1 * v x1 + p2 * v x2 + p3 * v x3 + p4 * (v x4 % 0x10000000000))
-let lemma_mod_264 x0 x1 x2 x3 x4 x5 x6 x7 x8 =
+let lemma_mod_264 x0 x1 x2 x3 x4 x5 x6 x7 x8 x9 =
   assert_norm(pow2 40 = 0x10000000000);
   assert_norm(pow2 16 = 0x10000);
   assert_norm(pow2 72 = 0x1000000000000000000);
   assert_norm(pow2 128 = 0x100000000000000000000000000000000);
   assert_norm(pow2 184 = 0x10000000000000000000000000000000000000000000000);
   assert_norm(pow2 264 = 0x1000000000000000000000000000000000000000000000000000000000000000000);
-  lemma_distr_4 0x1000000000000000000000000000000000000000000000000000000000000000000
-               (0x10000 * v x5) (0x1000000000000000000 * v x6) (0x100000000000000000000000000000000 * v x7) (0x10000000000000000000000000000000000000000000000 * v x8);
-  Math.Lemmas.lemma_mod_plus (v x0 + p1 * v x1 + p2 * v x2 + p3 * v x3 + p4 * v x4) (0x10000 * v x5 + 0x1000000000000000000 * v x6 + 0x100000000000000000000000000000000 * v x7 + 0x10000000000000000000000000000000000000000000000 * v x8) 0x1000000000000000000000000000000000000000000000000000000000000000000;
+  lemma_distr_5 0x1000000000000000000000000000000000000000000000000000000000000000000
+               (0x10000 * v x5) (0x1000000000000000000 * v x6) (0x100000000000000000000000000000000 * v x7) (0x10000000000000000000000000000000000000000000000 * v x8) (0x1000000000000000000000000000000000000000000000000000000000000 * v x9);
+  Math.Lemmas.lemma_mod_plus (v x0 + p1 * v x1 + p2 * v x2 + p3 * v x3 + p4 * v x4) (0x10000 * v x5 + 0x1000000000000000000 * v x6 + 0x100000000000000000000000000000000 * v x7 + 0x10000000000000000000000000000000000000000000000 * v x8 + 0x1000000000000000000000000000000000000000000000000000000000000 * v x9) 0x1000000000000000000000000000000000000000000000000000000000000000000;
   assert((v x0 + p1 * v x1 + p2 * v x2 + p3 * v x3 + p4 * v x4
-         + p5 * v x5 + p6 * v x6 + p7 * v x7 + p8 * v x8) % pow2 264
+         + p5 * v x5 + p6 * v x6 + p7 * v x7 + p8 * v x8 + p9 * v x9) % pow2 264
          = (v x0 + p1 * v x1 + p2 * v x2 + p3 * v x3 + p4 * v x4) % pow2 264);
   Math.Lemmas.lemma_mod_plus_distr_l (p4 * v x4) (v x0 + p1 * v x1 + p2 * v x2 + p3 * v x3) 0x1000000000000000000000000000000000000000000000000000000000000000000;
   assert_norm(p4 = pow2 224);
@@ -37,11 +41,11 @@ let lemma_mod_264 x0 x1 x2 x3 x4 x5 x6 x7 x8 =
   Math.Lemmas.modulo_lemma (v x0 + p1 * v x1 + p2 * v x2 + p3 * v x3 + p4 * (v x4 % 0x10000000000)) (pow2 264)
 
 val lemma_div_224:
-  x0:u56 -> x1:u56 -> x2:u56 -> x3:u56 -> x4:u56 -> x5:u56 -> x6:u56 -> x7:u56 -> x8:t ->
+  x0:u56 -> x1:u56 -> x2:u56 -> x3:u56 -> x4:u56 -> x5:u56 -> x6:u56 -> x7:u56 -> x8:u56 -> x9:u56 ->
   Lemma ((v x0 + p1 * v x1 + p2 * v x2 + p3 * v x3 + p4 * v x4
-         + p5 * v x5 + p6 * v x6 + p7 * v x7 + p8 * v x8) / pow2 224
-         = v x4 + p1 * v x5 + p2 * v x6 + p3 * v x7 + p4 * v x8)
-let lemma_div_224 x0 x1 x2 x3 x4 x5 x6 x7 x8 =
+         + p5 * v x5 + p6 * v x6 + p7 * v x7 + p8 * v x8 + p9 * v x9) / pow2 224
+         = v x4 + p1 * v x5 + p2 * v x6 + p3 * v x7 + p4 * v x8 + p5 * v x9)
+let lemma_div_224 x0 x1 x2 x3 x4 x5 x6 x7 x8 x9 =
   assert_norm(pow2 56  = 0x100000000000000);
   assert_norm(pow2 112 = 0x10000000000000000000000000000);
   assert_norm(pow2 168 = 0x1000000000000000000000000000000000000000000);
@@ -51,20 +55,16 @@ let lemma_div_224 x0 x1 x2 x3 x4 x5 x6 x7 x8 =
   assert_norm(pow2 392 = 0x100000000000000000000000000000000000000000000000000000000000000000000000000000000000000000000000000);
   assert_norm(pow2 448 = 0x10000000000000000000000000000000000000000000000000000000000000000000000000000000000000000000000000000000000000000)
 
-private
-let lemma_distr_5 x a b c d e : Lemma (x * (a + b + c + d + e) = x * a + x * b + x * c + x * d + x * e)
- = ()
-
 
 val lemma_div_24:
-  x0:u56 -> x1:u56 -> x2:u56 -> x3:u56 -> x4:u56 ->
-  Lemma ((v x0 + p1 * v x1 + p2 * v x2 + p3 * v x3 + p4 * v x4) / pow2 24
+  x0:u56 -> x1:u56 -> x2:u56 -> x3:u56 -> x4:u56 -> x5:UInt64.t{v x5 < 0x100} ->
+  Lemma ((v x0 + p1 * v x1 + p2 * v x2 + p3 * v x3 + p4 * v x4 + p5 * v x5) / pow2 24
          = v x0 / pow2 24 + (v x1 % pow2 24) * pow2 32
            + p1 * (v x1 / pow2 24 + (v x2 % pow2 24) * pow2 32)
            + p2 * (v x2 / pow2 24 + (v x3 % pow2 24) * pow2 32)
            + p3 * (v x3 / pow2 24 + (v x4 % pow2 24) * pow2 32)
-           + p4 * (v x4 / pow2 24))
-let lemma_div_24 x0 x1 x2 x3 x4 =
+           + p4 * (v x4 / pow2 24 + v x5 * pow2 32))
+let lemma_div_24 x0 x1 x2 x3 x4 x5 =
   assert_norm(pow2 24 = 0x1000000);
   assert_norm(pow2 32 = 0x100000000);
   assert_norm(pow2 56  = 0x100000000000000);
@@ -73,25 +73,26 @@ let lemma_div_24 x0 x1 x2 x3 x4 =
   assert_norm(pow2 224 = 0x100000000000000000000000000000000000000000000000000000000);
   Math.Lemmas.lemma_div_mod (v x0) (pow2 24);
   lemma_distr_5 0x1000000 (v x0 / pow2 24) (0x100000000 * v x1) (0x10000000000000000000000 * v x2) (0x1000000000000000000000000000000000000 * v x3) (0x100000000000000000000000000000000000000000000000000 * v x4);
-  Math.Lemmas.division_addition_lemma (v x0 % pow2 24) (pow2 24) ((v x0 / pow2 24)+(0x100000000 * v x1)+(0x10000000000000000000000 * v x2)+(0x1000000000000000000000000000000000000 * v x3)+(0x100000000000000000000000000000000000000000000000000 * v x4));
+  Math.Lemmas.division_addition_lemma (v x0 % pow2 24) (pow2 24) ((v x0 / pow2 24)+(0x100000000 * v x1)+(0x10000000000000000000000 * v x2)+(0x1000000000000000000000000000000000000 * v x3)+(0x100000000000000000000000000000000000000000000000000 * v x4)+(0x10000000000000000000000000000000000000000000000000000000000000000 * v x5));
   Math.Lemmas.small_division_lemma_1 (v x0 % pow2 24) (pow2 24);
   assert((v x0 + p1 * v x1 + p2 * v x2 + p3 * v x3 + p4 * v x4) / pow2 24
     = (v x0 / pow2 24 + (0x100000000 * v x1)+(0x10000000000000000000000 * v x2)+(0x1000000000000000000000000000000000000 * v x3)+(0x100000000000000000000000000000000000000000000000000 * v x4)));
     Math.Lemmas.lemma_div_mod (v x1) (pow2 24);
     Math.Lemmas.lemma_div_mod (v x2) (pow2 24);
     Math.Lemmas.lemma_div_mod (v x3) (pow2 24);
-    Math.Lemmas.lemma_div_mod (v x4) (pow2 24)
+    Math.Lemmas.lemma_div_mod (v x4) (pow2 24);
+    Math.Lemmas.lemma_div_mod (v x5) (pow2 24)
 
 
 val lemma_div_40:
-  x0:u56 -> x1:u56 -> x2:u56 -> x3:u56 -> x4:u56 ->
-  Lemma ((v x0 + p1 * v x1 + p2 * v x2 + p3 * v x3 + p4 * v x4) / pow2 40
+  x0:u56 -> x1:u56 -> x2:u56 -> x3:u56 -> x4:u56 -> x5:UInt64.t{v x5 < 0x1000000} ->
+  Lemma ((v x0 + p1 * v x1 + p2 * v x2 + p3 * v x3 + p4 * v x4 + p5 * v x5) / pow2 40
          = v x0 / pow2 40 + (v x1 % pow2 40) * pow2 16
            + p1 * (v x1 / pow2 40 + (v x2 % pow2 40) * pow2 16)
            + p2 * (v x2 / pow2 40 + (v x3 % pow2 40) * pow2 16)
            + p3 * (v x3 / pow2 40 + (v x4 % pow2 40) * pow2 16)
-           + p4 * (v x4 / pow2 40))
-let lemma_div_40 x0 x1 x2 x3 x4 =
+           + p4 * (v x4 / pow2 40 + v x5 * pow2 16))
+let lemma_div_40 x0 x1 x2 x3 x4 x5 =
   assert_norm(pow2 16 = 0x10000);
   assert_norm(pow2 32 = 0x100000000);
   assert_norm(pow2 40 = 0x10000000000);
@@ -101,11 +102,12 @@ let lemma_div_40 x0 x1 x2 x3 x4 =
   assert_norm(pow2 224 = 0x100000000000000000000000000000000000000000000000000000000);
   Math.Lemmas.lemma_div_mod (v x0) (pow2 40);
   lemma_distr_5 0x1000000 (v x0 / pow2 40) (0x10000 * v x1) (0x1000000000000000000 * v x2) (0x100000000000000000000000000000000 * v x3) (0x10000000000000000000000000000000000000000000000 * v x4);
-  Math.Lemmas.division_addition_lemma (v x0 % pow2 40) (pow2 40) ((v x0 / pow2 40)+(0x10000 * v x1)+(0x1000000000000000000 * v x2)+(0x100000000000000000000000000000000 * v x3)+(0x10000000000000000000000000000000000000000000000 * v x4));
+  Math.Lemmas.division_addition_lemma (v x0 % pow2 40) (pow2 40) ((v x0 / pow2 40)+(0x10000 * v x1)+(0x1000000000000000000 * v x2)+(0x100000000000000000000000000000000 * v x3)+(0x10000000000000000000000000000000000000000000000 * v x4)+(0x1000000000000000000000000000000000000000000000000000000000000 * v x5));
   Math.Lemmas.small_division_lemma_1 (v x0 % pow2 40) (pow2 40);
-  assert((v x0 + p1 * v x1 + p2 * v x2 + p3 * v x3 + p4 * v x4) / pow2 40
-    = (v x0 / pow2 40 + (0x10000 * v x1)+(0x1000000000000000000 * v x2)+(0x100000000000000000000000000000000 * v x3)+(0x10000000000000000000000000000000000000000000000 * v x4))); 
+  assert((v x0 + p1 * v x1 + p2 * v x2 + p3 * v x3 + p4 * v x4 + p5 * v x5) / pow2 40
+    = (v x0 / pow2 40 + (0x10000 * v x1)+(0x1000000000000000000 * v x2)+(0x100000000000000000000000000000000 * v x3)+(0x10000000000000000000000000000000000000000000000 * v x4)+(0x1000000000000000000000000000000000000000000000000000000000000 * v x5)));
     Math.Lemmas.lemma_div_mod (v x1) (pow2 40);
     Math.Lemmas.lemma_div_mod (v x2) (pow2 40);
     Math.Lemmas.lemma_div_mod (v x3) (pow2 40);
-    Math.Lemmas.lemma_div_mod (v x4) (pow2 40)
+    Math.Lemmas.lemma_div_mod (v x4) (pow2 40);
+    Math.Lemmas.lemma_div_mod (v x5) (pow2 40)
